merge piharmony branch

theories/pi/Congruence.v
@@ -1,6 +1,5 @@
-Require Import Coq.Program.Equality.
+Require Import Coq.Program.Equality Lia Arith.
 Require Import Relations Morphisms.
-
 From Must.pi Require Import Renamings.
 
 Reserved Notation "p ≡ q" (at level 70).
@@ -73,11 +72,90 @@ where "p ≡ q" := (cgr_step p q).
 
 #[global] Hint Constructors cgr_step:cgr_step_structure.
 
+(* Alternative definition of congruence step, better suited to prove that it's
+  a congruence *)
+Reserved Notation "p ≡ₐ q" (at level 70).
+Reserved Notation "p ≡g q" (at level 70).
+Inductive altcgr : proc -> proc -> Prop :=
+| altcgr_refl_step : forall p, p ≡ₐ p
+| altcgr_par_nil_step : forall p, 
+    (p ‖ 𝟘) ≡ₐ p
+| altcgr_par_nil_rev_step : forall p,
+    p ≡ₐ (p ‖ 𝟘)
+| altcgr_par_com_step : forall p q,
+    (p ‖ q) ≡ₐ (q ‖ p)
+| altcgr_par_assoc_step : forall p q r,
+    ((p ‖ q) ‖ r) ≡ₐ (p ‖ (q ‖ r))
+| altcgr_par_assoc_rev_step : forall p q r,
+    (p ‖ (q  ‖ r)) ≡ₐ ((p ‖ q) ‖ r)
+| altcgr_recursion_step : forall p q,
+    p ≡ₐ q -> (rec p) ≡ₐ (rec q)
+| altcgr_par_step : forall p q r,
+    p ≡ₐ q ->
+    (p ‖ r) ≡ₐ (q ‖ r)
+| altcgr_if_left_step : forall C p q q',
+    q ≡ₐ q' ->
+    (If C Then p Else q) ≡ₐ (If C Then p Else q')
+| altcgr_if_right_step : forall C p p' q,
+    p ≡ₐ p' ->
+    (If C Then p Else q) ≡ₐ (If C Then p' Else q)
+| altcgr_nu_nu_step : forall p,
+    (ν ν p) ≡ₐ (ν ν (p ⟨swap⟩))
+| altcgr_res_nil_step :
+    (ν 𝟘) ≡ₐ 𝟘
+| altcgr_res_nil_rev_step :
+    g 𝟘 ≡ₐ (ν 𝟘)
+| altcgr_res_step : forall p q,
+    p ≡ₐ q ->
+    (ν p) ≡ₐ (ν q)
+| altcgr_scope_step: forall (P Q:proc),
+    (ν (P ‖ (⇑ Q) )) ≡ₐ ((ν P) ‖ Q)
+| altcgr_scope_rev_step: forall (P Q:proc),
+    ((ν P) ‖ Q) ≡ₐ (ν (P ‖ (⇑ Q)))
+(* This rules is custom ; it's easily in the transitive closure of the standard
+ congruence. It actually implies altcgr_res_nil_step *)
+ (*
+| altcgr_scope_free: forall (p q : proc), p ≡ₐ ⇑ q -> ν p ≡ₐ q
+| altcgr_scope_free_rev: forall (p q : proc), p ≡ₐ ⇑ q -> q ≡ₐ ν p
+*)
+| altcgr_guard : forall (g1 g2 : gproc), g1 ≡g g2 -> g g1 ≡ₐ g g2
+| altcgr_trans : forall (p q r : proc) , p ≡ₐ q -> q ≡ₐ r -> p ≡ₐ r
+
+with altcgr_gstep : gproc -> gproc -> Prop :=
+| galtcgr_tau_step : forall p q,
+    p ≡ₐ q ->
+    (t • p) ≡g (t • q)
+| galtcgr_input_step : forall c p q,
+    p ≡ₐ q ->
+    (c ? p) ≡g (c ? q)
+| galtcgr_output_step : forall c v p q,
+    p ≡ₐ q ->
+    (c ! v • p) ≡g (c ! v • q)
+| galtcgr_choice_step : forall p1 q1 p2,
+    p1 ≡g q1 ->
+    (p1 + p2) ≡g (q1 + p2)
+| galtcgr_trans : forall (p q r : gproc), p ≡g q -> q ≡g r -> p ≡g r
+| galtcgr_choice_nil_step : forall p,
+    (p + 𝟘) ≡g p
+| galtcgr_choice_nil_rev_step : forall p,
+    p ≡g (p + 𝟘)
+| galtcgr_choice_com_step : forall p q,
+    (p + q) ≡g (q + p)
+| galtcgr_choice_assoc_step : forall p q r,
+    ((p + q) + r) ≡g (p + (q + r))
+| galtcgr_choice_assoc_rev_step : forall p q r,
+    (p + (q + r)) ≡g ((p + q) + r)
+| galtcgr_refl_step : forall p, p ≡g p
+| galtcgr_sym_step : forall p q, q ≡g p -> p ≡g q
+where "p ≡ₐ q" := (altcgr p q)
+and "p ≡g q" := (altcgr_gstep p q).
+#[local] Hint Constructors altcgr:alt_step_structure.
+
 #[global] Instance cgr_refl_step_is_refl : Reflexive cgr_step.
 Proof. intro. apply cgr_refl_step. Qed.
 #[global] Instance cgr_symm_step : Symmetric cgr_step.
 Proof. intros p q hcgr. induction hcgr; try solve [constructor; try exact IHhcgr].
-- rewrite <- (Swap_Proc_Involutive p) at 2. apply cgr_nu_nu_step.
+rewrite <- (Swap_Proc_Involutive p) at 2. apply cgr_nu_nu_step.
 Qed.
 
 Infix "≡" := cgr_step (at level 70).
@@ -88,7 +166,8 @@ Infix "≡*" := cgr (at level 70).
 #[global] Instance cgr_refl : Reflexive cgr.
 Proof. intros. constructor. apply cgr_refl_step. Qed.
 #[global] Instance cgr_symm : Symmetric cgr.
-Proof. intros p q hcgr. induction hcgr. constructor. apply cgr_symm_step. exact H. eapply t_trans; eauto. Qed.
+Proof. intros p q hcgr. induction hcgr. constructor. apply cgr_symm_step.
+exact H. eapply t_trans; eauto. Qed.
 #[global] Instance cgr_trans : Transitive cgr.
 Proof. intros p q r hcgr1 hcgr2. eapply t_trans; eauto. Qed.
 
@@ -99,6 +178,17 @@ Proof. repeat split.
        + apply cgr_refl.
        + apply cgr_symm.
        + apply cgr_trans.
+Qed.
+
+(* Transitive closure of congruence on guards only *)
+Definition guardcgr  :=
+  clos_trans proc (fun p1 p2 => exists g1 g2, p1 = g g1 /\ p2 = g g2 /\ p1 ≡ p2).
+
+#[local] Instance guard_cgr_refl : Symmetric guardcgr.
+Proof.
+  intros x y H. induction H.
+  - constructor. decompose record H. eauto with *.
+  - econstructor 2; eauto with *.
 Qed.
 
 (*the relation ≡* respects all the rules that ≡ respected*)
@@ -164,19 +254,45 @@ intros. induction H.
 constructor.
 - apply cgr_tau_step. exact H.
 - eauto with cgr_eq.
-Qed. 
+Qed.
+
+(* Stronger statement : congruences under tau preserve guards *)
+Lemma guardcgr_tau : forall p q, p ≡* q -> guardcgr (t • p) (t • q).
+Proof.
+intros. induction H.
+constructor.
+- eexists; eexists; repeat split. apply cgr_tau_step. exact H.
+- econstructor 2; eauto with cgr_eq.
+Qed.
+
 Lemma cgr_input : forall c p q, p ≡* q -> (c ? p) ≡* (c ? q).
 Proof.
 intros. induction H.
 - constructor. now apply cgr_input_step.
 - eauto with cgr_eq.
 Qed.
+
+Lemma guardcgr_input : forall c p q, p ≡* q -> guardcgr (c ? p) (c ? q).
+Proof.
+intros. induction H.
+- constructor. eexists; eexists; repeat split. now apply cgr_input_step.
+- econstructor 2; eauto with cgr_eq.
+Qed.
+
 Lemma cgr_output : forall c v p q, p ≡* q -> (c ! v • p) ≡* (c ! v • q).
 Proof.
 intros. induction H.
 - constructor. now apply cgr_output_step.
 - eauto with cgr_eq.
 Qed.
+
+Lemma guardcgr_output : forall c v p q, p ≡* q -> guardcgr (c ! v • p) (c ! v • q).
+Proof.
+intros. induction H.
+- constructor. eexists; eexists; repeat split. now constructor.
+- econstructor 2; eauto with cgr_eq.
+Qed.
+
 Lemma cgr_res : forall p q, p ≡* q -> (ν p) ≡* (ν q).
 Proof.
 intros. induction H.
@@ -219,12 +335,198 @@ intros. induction H.
 - constructor.  apply cgr_if_right_step. exact H.
 - eauto with cgr_eq.
 Qed.
-Lemma cgr_choice : forall p q r, (g p) ≡* (g q) -> p + r ≡* q + r.
+
+#[global] Instance altcgr_refl_step_is_refl : Reflexive altcgr.
+Proof. intro. apply altcgr_refl_step. Qed.
+
+#[global] Instance altcgr_grefl_step_is_refl : Reflexive altcgr_gstep.
+Proof. intro. constructor. Qed.
+
+#[local] Instance altcgr_symm_step : Symmetric altcgr.
+Proof. intros p q hcgr. induction hcgr; try solve [constructor; try exact IHhcgr];
+try solve[now (do 3 (try constructor))].
+- rewrite <- (Swap_Proc_Involutive p) at 2. apply altcgr_nu_nu_step.
+- constructor. now constructor.
+- econstructor; eauto.
+Qed.
+
+(* The lemmas on renaming suffice for all of the treatment, except recursive variables. *)
+Instance RenProperStep : Proper (eq ==> (pointwise_relation _ eq) ==> cgr_step ==> cgr_step) ren2.
 Proof.
-intros. dependent induction H.
-- constructor. apply cgr_choice_step. exact H.
-- etransitivity. apply (IHclos_trans1 p q). reflexivity.
-Admitted.
+intros sp' sp Hp s' s Hs q1 q2 Hq. rewrite Hs. clear Hs s'. subst.
+  revert sp s.
+  induction Hq; intros; try solve [asimpl; auto with cgr_step_structure].
+  - asimpl. apply cgr_choice_step. apply IHHq.
+  - asimpl. simpl. change (idsRen >> sp) with sp.
+    replace (ren_proc sp (1 .: (0 .: (fun x => S (S (s x))))) p) 
+      with  ((ren_proc sp (0 .: (1 .: (fun x => S (S (s x))))) p) ⟨swap⟩)
+      by now asimpl.
+    apply cgr_nu_nu_step.
+  - unfold ren2. simpl. rewrite permute_ren. exact (cgr_scope_step _ _).
+  - unfold ren2. simpl. rewrite permute_ren. exact (cgr_scope_rev_step _ _).
+Qed.
+
+Instance RenProper : Proper (eq ==> (pointwise_relation _ eq) ==> cgr ==> cgr) ren2.
+Proof.
+intros sp' sp Hp s' s Hs q1 q2 Hq. rewrite Hs.
+induction Hq as [p q base_case | p r q transitivity_case].
+- subst. apply t_step. apply RenProperStep; trivial. intro n; trivial.
+- subst. now rewrite IHtransitivity_case.
+Qed.
+
+
+(* Equivalence between the two definitions *)
+
+Scheme proc_ind2 := Induction for proc Sort Prop
+  with gproc_ind2 := Induction for gproc Sort Prop.
+
+Lemma cgr_step_altcgr p q: cgr_step p q -> altcgr p q.
+Proof.
+revert q.
+induction p using proc_ind2 with (P0 :=
+  (fun gp => forall gq, cgr_step (g gp) (g gq) -> altcgr_gstep gp gq));
+intros q Hq;
+try (solve[inversion Hq; subst; eauto with *; do 2 try constructor; eauto]).
+inversion Hq; subst; eauto with *;
+try (solve[inversion Hq; subst; eauto with *; do 2 try constructor; eauto]).
+constructor. now apply IHp.
+Qed.
+
+Lemma cgr_altcgr p q: cgr p q -> altcgr p q.
+Proof. intro H. induction H; eauto using cgr_step_altcgr with *. Qed.
+
+Scheme altcgr_ind2 := Induction for altcgr Sort Prop
+  with galtcgr_ind2 := Induction for altcgr_gstep Sort Prop.
+
+Combined Scheme altcgr_mutind from altcgr_ind2,galtcgr_ind2.
+
+Lemma guardcgr_choice_step p1 q1 p2: guardcgr (g p1) (g q1) ->
+  guardcgr (g (p1 + p2)) (g (q1 + p2)).
+Proof.
+  intros H%clos_trans_tn1. apply clos_tn1_trans. dependent induction H.
+  - constructor. decompose record H; subst.
+    eexists; eexists; repeat split. now constructor.
+  - decompose record H; subst; clear H. inversion H2; subst.
+    econstructor 2; eauto.
+    eexists; eexists; repeat split. now constructor.
+Qed.
+
+Lemma guardcgr_cgr p q : guardcgr p q -> cgr p q.
+Proof. intro H. induction H; eauto with *; decompose record H; now constructor. Qed.
+
+(* The following goes through because we strengthen the conclusion on guards *)
+Lemma altcgr_cgr :
+  (forall p q, altcgr p q -> p ≡* q) /\
+  (forall gp gq, altcgr_gstep gp gq -> guardcgr gp gq).
+Proof.
+apply altcgr_mutind; try solve [repeat constructor; eauto with *]; intros.
+- now apply cgr_recursion.
+- now apply cgr_par.
+- now apply cgr_if_left.
+- now apply cgr_if_right.
+- now apply cgr_res.
+- now apply guardcgr_cgr.
+- eauto with *.
+- now apply guardcgr_tau.
+- now apply guardcgr_input.
+- now apply guardcgr_output.
+- now apply guardcgr_choice_step.
+- intros. now apply t_trans with (g q).
+- now symmetry.
+Qed.
+
+(* Being syntactically equivalent to a guard, hidden under parallels and unnecessary restrictions *)
+Fixpoint sguard (g0 : gproc) (p : proc) := match p with
+| (p ‖ q) => (sguard 𝟘 p /\ sguard g0 q) \/ (sguard 𝟘 q /\ sguard g0 p)
+| (ν p) => sguard (⇑ g0) p
+| g p => p ≡g g0
+| _ => False
+end.
+
+(* congruence is preserved by renamings *)
+Lemma ren2_altcgr:
+  (forall p1 p2, p1 ≡ₐ p2 -> forall s1 s2, ren2 s1 s2 p1 ≡ₐ ren2 s1 s2 p2) /\
+  (forall g1 g2, g1 ≡g g2 -> forall s1 s2, ren2 s1 s2 g1 ≡g ren2 s1 s2 g2).
+Proof.
+apply altcgr_mutind; intros; asimpl; simpl; try solve [constructor; eauto with *].
+- (* unification issue *)
+  generalize (altcgr_nu_nu_step (ren2 s1 (0 .: (1 .: (fun x : nat => S (S (s2 x))))) p)).
+  now asimpl.
+- generalize (altcgr_scope_step (ren2 s1 (0 .: s2 >> S) P) (ren2 s1 s2 Q)).
+  now asimpl.
+- generalize (altcgr_scope_rev_step (ren2 s1 (0 .: s2 >> S) P) (ren2 s1 s2 Q)).
+  now asimpl.
+- eapply altcgr_trans; eauto.
+- eapply galtcgr_trans; eauto.
+Qed.
+
+Lemma sguard_cgr_proper p g g': sguard g p -> g ≡g g' -> sguard g' p.
+Proof.
+revert g g'. induction p; simpl; intuition.
+- left. intuition. eauto with *.
+- right. intuition. eauto with *.
+- eapply IHp; [eassumption|]. now apply ren2_altcgr.
+- apply galtcgr_trans with g1; trivial.
+Qed.
+
+Lemma ren2_sguard p g s1 s2 : sguard g p -> sguard (ren2 s1 s2 g) (ren2 s1 s2 p).
+Proof.
+revert g s1 s2. induction p; intros g s1 s2; simpl; intuition.
+- left. split; [now apply (IHp1 𝟘)| now apply IHp2].
+- right. split; [now apply (IHp2 𝟘) | now apply IHp1].
+- revert H. rewrite <- permute_ren_guard. apply IHp; trivial.
+- now apply ren2_altcgr.
+Qed.
+
+Definition shift_down_proc := ren2 ids pred.
+
+Lemma shift_down_up_proc : forall p : proc, shift_down_proc (⇑ p) = p.
+Proof. now asimpl. Qed.
+
+Definition shift_down_gproc := ren2 ids pred : gproc -> gproc.
+Lemma shift_down_up_gproc : forall p : gproc, shift_down_gproc (⇑ p) = p.
+Proof. now asimpl. Qed.
+
+Instance RenProperAltcgr : Proper (eq ==> (eq) ==> altcgr ==> altcgr) ren2.
+Proof. intros ?????????. subst. now apply ren2_altcgr. Qed.
+
+Lemma altcgr_guard_proper (p0 p1 : proc) (g0 : gproc) : (p0 ≡ₐ p1) -> sguard g0 p0
+  -> sguard g0 p1.
+Proof.
+intro H. dependent induction H generalizing g0; simpl; try solve[constructor]; auto with *;
+intuition; simpl; eauto with *.
+- eapply sguard_cgr_proper; eauto.
+- replace (⇑ (⇑ g0)) with ((⇑ (⇑ g0)) ⟨ swap ⟩) by (now asimpl).
+  now apply ren2_sguard.
+- rewrite <- (shift_down_up_gproc g0), <- (shift_down_up_gproc 𝟘).
+  change (⇑ 𝟘) with 𝟘. now apply ren2_altcgr.
+- change 𝟘 with (⇑ 𝟘). now apply ren2_altcgr.
+- left. split; trivial.
+  rewrite <- (shift_down_up_gproc g0), <- (shift_down_up_proc Q).
+  now apply ren2_sguard.
+- right. split; trivial. change 𝟘 with (⇑ 𝟘) in H.
+  rewrite <- (shift_down_up_proc Q), <- (shift_down_up_gproc 𝟘).
+  now apply ren2_sguard.
+- left. split; trivial. now apply ren2_sguard.
+- right. split; trivial. change 𝟘 with (⇑ 𝟘). now apply ren2_sguard.
+- apply galtcgr_trans with g1; trivial. now apply galtcgr_sym_step.
+Qed.
+
+(* The congruence between guards, is no stronger than the congruence over guards *)
+Lemma altcgr_guard_rev g1 g2: g g1 ≡ₐ g g2 -> g1 ≡g g2.
+Proof.
+intro Ha. inversion Ha; subst; [constructor|auto|].
+apply (altcgr_guard_proper q (g g1) g2); [now symmetry|].
+apply (altcgr_guard_proper (g g2) q g2); [now symmetry|].
+constructor.
+Qed.
+
+(* Choice respects ≡* *)
+Lemma cgr_choice : forall p q r, g p ≡* g q -> p + r ≡* q + r.
+Proof.
+intros p q r H%cgr_altcgr%altcgr_guard_rev.
+apply altcgr_cgr. now do 2 constructor.
+Qed.
 
 (* The if of processes respects ≡* *)
 Lemma cgr_full_if : forall C p p' q q', p ≡* p' -> q ≡* q' -> (If C Then p Else q) ≡* (If C Then p' Else q').
@@ -280,30 +582,6 @@ Qed.
 
 (* The old Congruence lemmas can now be restated using Autosubst's help.
    This still requires some technical work and lemmas on substitutions. *)
-
-(* The lemmas on renaming suffice for all of the treatment, except recursive variables. *)
-Instance RenProperStep : Proper (eq ==> (pointwise_relation _ eq) ==> cgr_step ==> cgr_step) ren2.
-Proof.
-intros sp' sp Hp s' s Hs q1 q2 Hq. rewrite Hs. clear Hs s'. subst.
-  revert sp s.
-  induction Hq; intros; try solve [asimpl; auto with cgr_step_structure].
-  - asimpl. apply cgr_choice_step. apply IHHq.
-  - asimpl. simpl. change (idsRen >> sp) with sp.
-    replace (ren_proc sp (1 .: (0 .: (fun x => S (S (s x))))) p) 
-      with  ((ren_proc sp (0 .: (1 .: (fun x => S (S (s x))))) p) ⟨swap⟩)
-      by now asimpl.
-    apply cgr_nu_nu_step.
-  - unfold ren2. simpl. rewrite permute_ren. exact (cgr_scope_step _ _).
-  - unfold ren2. simpl. rewrite permute_ren. exact (cgr_scope_rev_step _ _).
-Qed.
-
-Instance RenProper : Proper (eq ==> (pointwise_relation _ eq) ==> cgr ==> cgr) ren2.
-Proof.
-intros sp' sp Hp s' s Hs q1 q2 Hq. rewrite Hs.
-induction Hq as [p q base_case | p r q transitivity_case].
-- subst. apply t_step. apply RenProperStep; trivial. intro n; trivial.
-- subst. now rewrite IHtransitivity_case.
-Qed.
 
 (* In order to treat recursive variables, we need more subtle instances on substitutions *)
 Definition eq_up_to_cgr f g := forall x :nat, f x ≡* g x.
